Views: remove length index, make it a field instead

dist/Kuiper_ArrayView_Test_EvenOdds4.cu
@@ -4,29 +4,3 @@
 
 uint32_t Kuiper_ArrayView_Test_EvenOdds4_x = 1U;
 
-uint32_t Kuiper_ArrayView_Test_EvenOdds4_foo_even(uint32_t *a)
-{
-  return a[20U];
-}
-
-uint32_t Kuiper_ArrayView_Test_EvenOdds4_foo_odd(uint32_t *a)
-{
-  return a[21U];
-}
-
-uint32_t Kuiper_ArrayView_Test_EvenOdds4_foo_even_over_raw(uint32_t *a)
-{
-  return a[20U];
-}
-
-uint32_t Kuiper_ArrayView_Test_EvenOdds4_foo_odd_over_raw(uint32_t *a)
-{
-  return a[21U];
-}
-
-uint32_t Kuiper_ArrayView_Test_EvenOdds4_test_over_raw(uint32_t *a)
-{
-  uint32_t *a_ = a;
-  return a_[20U] + a_[21U];
-}
-
