dist/Kuiper_ArrayView_Test_EvenOdds4.h
@@ -7,16 +7,6 @@
 
 extern uint32_t Kuiper_ArrayView_Test_EvenOdds4_x;
 
-uint32_t Kuiper_ArrayView_Test_EvenOdds4_foo_even(uint32_t *a);
-
-uint32_t Kuiper_ArrayView_Test_EvenOdds4_foo_odd(uint32_t *a);
-
-uint32_t Kuiper_ArrayView_Test_EvenOdds4_foo_even_over_raw(uint32_t *a);
-
-uint32_t Kuiper_ArrayView_Test_EvenOdds4_foo_odd_over_raw(uint32_t *a);
-
-uint32_t Kuiper_ArrayView_Test_EvenOdds4_test_over_raw(uint32_t *a);
-
 
 #define Kuiper_ArrayView_Test_EvenOdds4_H_DEFINED
 #endif /* Kuiper_ArrayView_Test_EvenOdds4_H */
