src/examples/Kuiper.ArrayView.Test.EvenOdds.fst
@@ -14,8 +14,9 @@ module IView = Kuiper.IView
 module SZ    = FStar.SizeT
 
 noextract
-let even_view et len : aview et len (lseq et ((len + 1) / 2)) = {
+let even_view et (len : nat) : aview et (lseq et ((len + 1) / 2)) = {
   iview = {
+    len;
     sch = {
       ait = natlt ((len + 1) / 2);
       ait_enum = solve;
@@ -31,8 +32,9 @@ let even_view et len : aview et len (lseq et ((len + 1) / 2)) = {
 }
 
 noextract
-let odd_view et len : aview et len (lseq et (len / 2)) = {
+let odd_view et (len : nat) : aview et (lseq et (len / 2)) = {
   iview = {
+    len;
     sch = {
       ait = natlt (len / 2);
       ait_enum = solve;
@@ -47,9 +49,13 @@ let odd_view et len : aview et len (lseq et (len / 2)) = {
   igm = solve;
 }
 
+(* Somehow generate these automatically for constants? *)
 inline_for_extraction noextract
-instance _cview_even #et (#len : erased nat{SZ.fits len}) : IView.ciview (even_view et len).iview = {
-  fits = ();
+instance concrete_sz_100 : concrete_sz 100 = { x = 100sz }
+
+inline_for_extraction noextract
+instance _cview_even #et (len : erased nat) (sz_len : concrete_sz len) : IView.ciview (even_view et len).iview = {
+  clen = sz_len.x;
   sch = {
     cit  = szlt ((len + 1) / 2);
     bij  = natural;
@@ -64,8 +70,8 @@ instance _cview_even #et (#len : erased nat{SZ.fits len}) : IView.ciview (even_v
 }
 
 inline_for_extraction noextract
-instance _cview_odd #et (#len : erased nat{SZ.fits len}) : IView.ciview (odd_view et len).iview = {
-  fits = ();
+instance _cview_odd #et (len : erased nat) (sz_len : concrete_sz len) : IView.ciview (odd_view et len).iview = {
+  clen = sz_len.x;
   sch = {
     cit  = szlt (len / 2);
     bij  = natural;
@@ -82,11 +88,13 @@ instance _cview_odd #et (#len : erased nat{SZ.fits len}) : IView.ciview (odd_vie
 fn foo_even (a : varray (even_view u32 100))
   (#v0 : erased (lseq u32 50))
   preserves gpu
-  requires a |-> v0
-  returns u32
-  ensures  a |-> v0
+  preserves a |-> v0
+  returns   u32
 {
-  varray_read a 10sz;
+  varray_read #_ #_ #_ #(_cview_even #_ _ solve) a 10sz;
+  // Bad tc resolution due to the different shape
+  // of the lengths in lseq. The one for a gets simplified
+  // to 50, which does not unify with (?u+1)/2 in the instance.
 }
 
 fn foo_odd (a : varray (odd_view u32 100))
@@ -96,7 +104,7 @@ fn foo_odd (a : varray (odd_view u32 100))
   returns u32
   ensures  a |-> v0
 {
-  varray_read a 10sz;
+  varray_read #_ #_ #_ #(_cview_odd #_ _ solve) a 10sz;
 }
 
 fn test (a : gpu_array u32 100)
