src/examples/Kuiper.ArrayView.Test.EvenOdds3.fst
@@ -18,9 +18,10 @@ module SZ    = FStar.SizeT
 // Can we use divup here? It seems much harder on Z3.
 noextract
 let strided_view et (len : nat) (stride : nat) (offset : natlt stride) :
-  aview et len (lseq et ((len + stride - 1 - offset) / stride))
+  aview et (lseq et ((len + stride - 1 - offset) / stride))
 = {
   iview = {
+    len;
     sch = {
       ait = natlt ((len + stride - 1 - offset) / stride);
       ait_enum = solve;
@@ -35,16 +36,17 @@ let strided_view et (len : nat) (stride : nat) (offset : natlt stride) :
   igm = solve;
 }
 
-let even_view et len : aview et len _ = strided_view et len 2 0
-let odd_view  et len : aview et len _ = strided_view et len 2 1
+let even_view et len : aview et _ = strided_view et len 2 0
+let odd_view  et len : aview et _ = strided_view et len 2 1
 
 inline_for_extraction noextract
 instance _cview_strided
    (#et : Type) (#len : erased nat{SZ.fits len})
+   {| sz_len : concrete_sz len |}
    (stride : sz) (offset : szlt stride)
 : IView.ciview (strided_view et len stride offset).iview
 = {
-  fits = ez;
+  clen = sz_len.x;
   sch = {
     cit  = szlt ((len + stride - 1 - offset) / stride);
     bij  = natural;
@@ -59,30 +61,33 @@ instance _cview_strided
 }
 
 inline_for_extraction noextract
-instance _cview_even #et (#len : erased nat{SZ.fits len}) : IView.ciview (even_view et len).iview =
+instance _cview_even #et (#len : erased nat{SZ.fits len}) {| concrete_sz len |} : IView.ciview (even_view et len).iview =
   _cview_strided #et #len 2sz 0sz
 
 inline_for_extraction noextract
-instance _cview_odd #et (#len : erased nat{SZ.fits len}) : IView.ciview (odd_view et len).iview =
+instance _cview_odd #et (#len : erased nat{SZ.fits len}) {| concrete_sz len |} : IView.ciview (odd_view et len).iview =
   _cview_strided #et #len 2sz 1sz
 
 (* What is happening?!?! Why isn't this obvious? *)
 
-let _wat_even (#len : nat{SZ.fits len}) :
+let _wat_even (#len : nat{SZ.fits len}) {| concrete_sz len |} :
   Lemma (reveal (_cview_even #u32 #len).sch.bij == fin_size_t_bij ((len + 2 - 1 - 0) / 2))
         [SMTPat (_cview_even #u32 #len)]
 = assert_norm (reveal (_cview_even #u32 #len).sch.bij == fin_size_t_bij ((len + 2 - 1 - 0) / 2))
 
-let _wat_odd (#len : nat{SZ.fits len}) :
+let _wat_odd (#len : nat{SZ.fits len}) {| concrete_sz len |}:
   Lemma (reveal (_cview_odd #u32 #len).sch.bij == fin_size_t_bij ((len + 2 - 1 - 1) / 2))
         [SMTPat (_cview_odd #u32 #len)]
 = () // assert_norm (reveal (_cview_odd #u32 #len).bij == fin_size_t_bij ((len + 2 - 1 - 1) / 2))
 
-let _sanity1 (#len : nat{SZ.fits len}) (x : szlt ((len + 1) / 2)) : Lemma (ci_to_ai (even_view u32 len) x == SZ.v x)
+let _sanity1 (#len : nat{SZ.fits len}) (x : szlt ((len + 1) / 2)) {| concrete_sz len |} : Lemma (ci_to_ai (even_view u32 len) x == SZ.v x)
   = ()
 
-let _sanity2 (#len : nat{SZ.fits len}) (x : szlt (len / 2)) : Lemma (ci_to_ai (odd_view u32 len) x == SZ.v x)
+let _sanity2 (#len : nat{SZ.fits len}) (x : szlt (len / 2)) {| concrete_sz len |}: Lemma (ci_to_ai (odd_view u32 len) x == SZ.v x)
   = ()
+
+inline_for_extraction noextract
+instance _ : concrete_sz 100 = { x = 100sz; }
 
 fn foo_even (a : varray (even_view u32 100))
   (#v0 : erased (lseq u32 50))
@@ -91,7 +96,7 @@ fn foo_even (a : varray (even_view u32 100))
   returns u32
   ensures  a |-> v0
 {
-  varray_read a 10sz;
+  varray_read #_ #_ #_ #_cview_even a 10sz;
 }
 
 fn foo_odd (a : varray (odd_view u32 100))
@@ -101,7 +106,7 @@ fn foo_odd (a : varray (odd_view u32 100))
   returns u32
   ensures  a |-> v0
 {
-  varray_read a 10sz;
+  varray_read #_ #_ #_ #_cview_odd a 10sz;
 }
 
 let vw = sum_aview (even_view u32 100) (odd_view u32 100)
@@ -207,8 +212,8 @@ fn test_write (a : gpu_array u32 100)
     ;
   // Note: that doesn't happen if we use split2_, the ghost version
 
-  varray_write vl 10sz 42ul;
-  varray_write vr 20sz 43ul;
+  varray_write #_ #_ #_ #_cview_even vl 10sz 42ul;
+  varray_write #_ #_ #_ #_cview_odd  vr 20sz 43ul;
 
   let va = varray_join2 vl vr;
 
