src/lib/views/Kuiper.IView.fsti
@@ -5,6 +5,7 @@ module Kuiper.IView
 #lang-pulse
 
 open Kuiper
+open Kuiper.Len
 open Kuiper.Bijection
 open Kuiper.Injection
 open FStar.Tactics.Typeclasses { no_method }
@@ -38,35 +39,41 @@ let raw_aiview_schema (len : nat) : aiview_schema = {
 [@@erasable]
 noeq
 inline_for_extraction noextract
-type aiview (len : erased nat) = {
+type aiview = {
+  len  : nat;
   sch  : aiview_schema;
   step : aiview_step sch.ait (natlt len);
 }
 
 unfold
-instance enumerable_aiview_ait (#len:nat) (vw : aiview len)
+instance has_len_aiview : has_len aiview = {
+  len = (fun vw -> vw.len);
+}
+
+unfold
+instance enumerable_aiview_ait (vw : aiview)
   : Enumerable.enumerable vw.sch.ait
 = vw.sch.ait_enum
 
-let is_full_view (#len : nat) (avw : aiview len) : prop =
+let is_full_view (avw : aiview) : prop =
   is_surj avw.step.imap.f
 
-let is_full_view_lempat (#len : nat) (avw : aiview len { is_full_view avw })
-     (i : natlt len)
+let is_full_view_lempat (avw : aiview { is_full_view avw })
+     (i : natlt avw.len)
   : Lemma (in_image avw.step.imap.f i)
           [SMTPat (in_image avw.step.imap.f i)]
   = ()
 
 (* Will this be useful? *)
 val full_iff_cardinal
-  (#len : nat)
-  (vw : aiview len)
-  : Lemma (is_full_view vw <==> vw.sch.ait_enum._cardinal == len)
+  (vw : aiview)
+  : Lemma (is_full_view vw <==> vw.sch.ait_enum._cardinal == vw.len)
           [SMTPat (is_full_view vw)]
 
 (* Nothing fancy here. *)
 inline_for_extraction noextract
-let raw_view (#len : erased nat) : aiview len = {
+let raw_view (#len : erased nat) : aiview = {
+  len  = len;
   sch  = raw_aiview_schema len;
   step = { imap = inj_id; };
 }
@@ -124,21 +131,21 @@ class ciview_step
 
 (* What it means for an indexing view to be concretizable, i.e. executable. *)
 inline_for_extraction noextract
-class ciview (#len : erased nat) (avw : aiview len) =
+class ciview (avw : aiview) =
 {
   [@@@no_method]
-  fits : squash (SZ.fits len); // Hmm.. feels a bit out of place?
+  clen : (clen : SZ.t {SZ.v clen == avw.len});
 
   [@@@no_method]
   sch  : ciview_schema avw.sch;
 
   [@@@no_method]
-  step : ciview_step sch (raw_ciview_schema len) avw.step;
+  step : ciview_step sch (raw_ciview_schema avw.len) avw.step;
 }
 
 inline_for_extraction noextract
 instance concrete_raw_view (#len : nat{SZ.fits len}) : ciview (raw_view #len) = {
-  fits = ();
+  clen = SZ.uint_to_t len; // weird
   sch  = raw_ciview_schema len;
   step = {
     cimap  = inj_id;
@@ -158,12 +165,13 @@ let inj_bij' (#a #b : Type) (bij : a =~ b) : (b @~> a) =
   is_inj = ez;
 }
 
-let reindex_view (#len : nat)
-  (vw : aiview len)
+let reindex_view
+  (vw : aiview)
   (#ait' : Type)
   {| Enumerable.enumerable ait' |}
   (bij : vw.sch.ait =~ ait')
-  : aiview len = {
+  : aiview = {
+  len = vw.len;
   sch = {
     ait      = ait';
     ait_enum = solve;
@@ -175,39 +183,36 @@ let reindex_view (#len : nat)
 }
 
 let it_to_nat
-  (#len:nat)
-  (vw : aiview len)
+  (vw : aiview)
   (i : vw.sch.ait)
-  : GTot (natlt len)
+  : GTot (natlt vw.len)
   = i |~> vw.step.imap
 
 let it_of_nat
-  (#len:nat)
-  (vw : aiview len)
-  (i: natlt len{FStar.Functions.in_image vw.step.imap.f i})
+  (vw : aiview)
+  (i: natlt vw.len{FStar.Functions.in_image vw.step.imap.f i})
   : GTot vw.sch.ait
   = i <~| vw.step.imap
 
 let ci_to_ai
-  (#len:nat)
-  (vw : aiview len) {| cw : ciview vw |}
+  (vw : aiview) {| cw : ciview vw |}
   (i : cw.sch.cit)
   : GTot vw.sch.ait
   = let open Kuiper.Bijection in
     i <~| cw.sch.bij
 
 let ai_to_ci
-  (#len:nat)
-  (vw : aiview len) {| cw : ciview vw |}
+  (vw : aiview) {| cw : ciview vw |}
   (i : vw.sch.ait)
   : GTot cw.sch.cit
   = let open Kuiper.Bijection in
     i |~> cw.sch.bij
 
-let sum_aiview (#len : nat)
-  (vw1 vw2 : aiview len)
+let sum_aiview
+  (vw1 vw2 : aiview) // { vw1.len == vw2.len })
   (#_ : squash (no_overlap vw1.step.imap.f vw2.step.imap.f))
-  : aiview len = {
+  : aiview = {
+  len = max vw1.len vw2.len;
   sch = {
     ait      = either vw1.sch.ait vw2.sch.ait;
     ait_enum = solve;
