src/lib/views/Kuiper.View.fst
@@ -6,19 +6,19 @@ open Kuiper
 open Kuiper.Bijection
 module F = FStar.FunctionalExtensionality
 
-let to_from (#a:Type) (#len:nat) (#st:Type)
-  (vw : aview a len st { is_full_view vw })
-  (s : lseq a len)
+let to_from (#a:Type) (#st:Type)
+  (vw : aview a st { is_full_view vw })
+  (s : lseq a (len vw))
   : Lemma (ensures to_seq vw (from_seq vw s) == s)
           [SMTPat (to_seq vw (from_seq vw s))]
   = let _ = vw.igm.bij.gg (F.on_g vw.iview.sch.ait <| fun i -> s @! it_to_nat vw i) in
     (* funny, mentioning the term above (= from_seq vw s) makes the proof work. *)
-    let aux (i : natlt len)
+    let aux (i : natlt (len vw))
       : Lemma (to_seq vw (from_seq vw s) @! i == s @! i) =
       calc (==) {
         to_seq vw (from_seq vw s) @! i;
         == {}
-        Seq.init_ghost len (fun j -> reveal (vw.igm.acc (from_seq vw s) (it_of_nat vw j))) @! i;
+        Seq.init_ghost (len vw) (fun (j : natlt (len vw)) -> reveal (vw.igm.acc (from_seq vw s) (it_of_nat vw j))) @! i;
         == {}
         reveal (vw.igm.acc (from_seq vw s) (it_of_nat vw i));
         == {}
@@ -38,8 +38,8 @@ let to_from (#a:Type) (#len:nat) (#st:Type)
     Classical.forall_intro aux;
     assert (Seq.equal s (to_seq vw (from_seq vw s)))
 
-let from_to (#a:Type) (#len:nat) (#st:Type)
-  (vw : aview a len st { is_full_view vw })
+let from_to (#a:Type) (#st:Type)
+  (vw : aview a st { is_full_view vw })
   (v : st)
   : Lemma (ensures from_seq vw (to_seq vw v) == v)
           [SMTPat (from_seq vw (to_seq vw v))]
@@ -76,32 +76,34 @@ let from_to (#a:Type) (#len:nat) (#st:Type)
     rhs;
   }
 
-let to_seq_upd (#a:Type) (#len:nat) (#st:Type)
-  (vw : aview a len st { is_full_view vw })
+#push-options "--retry 5" // flaky, but fast when it works
+let to_seq_upd (#a:Type) (#st:Type)
+  (vw : aview a st { is_full_view vw })
   (v : st)
   (i : vw.iview.sch.ait)
   (x : a)
   : Lemma (ensures to_seq vw (vw.igm.upd v i x) == Seq.upd (to_seq vw v) (it_to_nat vw i) x)
           [SMTPat (to_seq vw (vw.igm.upd v i x))]
 =
-  let aux (idx : natlt len)
+  let aux (idx : natlt (len vw))
     : Lemma (to_seq vw (vw.igm.upd v i x) @! idx == Seq.upd (to_seq vw v) (it_to_nat vw i) x @! idx) =
     vw.igm.l2 (it_of_nat vw idx) v x;
     // calc (==) {
     //   to_seq vw (vw.igm.upd v i x) @! idx;
     //   == {}
-    //   Seq.init_ghost len (fun j -> reveal (vw.igm.acc (vw.igm.upd v i x) (it_of_nat vw j))) @! idx;
-    //   == {}
-    //   reveal (vw.igm.acc (vw.igm.upd v i x) (it_of_nat vw idx));
-    //   == { vw.igm.l2 (it_of_nat vw idx) v x }
-    //   if FStar.StrongExcludedMiddle.strong_excluded_middle (it_of_nat vw idx == i)
-    //   then x
-    //   else reveal (vw.igm.acc v (it_of_nat vw idx));
-    //   == {}
+    //   // Seq.init_ghost (len vw) (fun (j : natlt (len vw)) -> reveal (vw.igm.acc (vw.igm.upd v i x) (it_of_nat vw j))) @! idx;
+    //   // == {}
+    //   // reveal (vw.igm.acc (vw.igm.upd v i x) (it_of_nat vw idx));
+    //   // == { vw.igm.l2 (it_of_nat vw idx) v x }
+    //   // if FStar.StrongExcludedMiddle.strong_excluded_middle (it_of_nat vw idx == i)
+    //   // then x
+    //   // else reveal (vw.igm.acc v (it_of_nat vw idx));
+    //   // == {}
     //   Seq.upd (to_seq vw v) (it_to_nat vw i) x @! idx;
-    // }
+    // };
     ()
   in
   Classical.forall_intro aux;
   assert (to_seq vw (vw.igm.upd v i x) `Seq.equal` Seq.upd (to_seq vw v) (it_to_nat vw i) x) ;
   ()
+#pop-options
