src/lib/views/Kuiper.View.fsti
@@ -3,6 +3,7 @@ module Kuiper.View
 #lang-pulse
 
 open Kuiper
+open Kuiper.Len
 open Kuiper.GhostMap { is_ghost_map }
 open Kuiper.Bijection
 open Kuiper.Injection
@@ -12,35 +13,45 @@ module SZ = FStar.SizeT
 
 [@@erasable]
 noeq
-type aview (et : Type) (len : nat) (st : Type0) = {
+type aview (et : Type) (st : Type0) = {
   (* An indexing view. *)
-  iview : aiview len;
+  iview : aiview;
 
   (* The high-level spec type is a container, roughly a ghost function ait -> et *)
   igm  : is_ghost_map st iview.sch.ait et;
 }
 
 unfold
-instance enumerable_view_ait (#et:Type) (#len: erased nat) (#st:Type0)
-  (vw : aview et len st)
+instance has_len_aview (et st : Type) : has_len (aview et st) = {
+  len = (fun vw -> vw.iview.len);
+}
+
+let _helper (et st : Type) (vw : aview et st)
+  : Lemma (len vw == vw.iview.len)
+          [SMTPat (len vw)]
+  = ()
+
+unfold
+instance enumerable_view_ait (#et:Type) (#st:Type0)
+  (vw : aview et st)
   : Enumerable.enumerable vw.iview.sch.ait
 = vw.iview.sch.ait_enum
 
 unfold
-instance is_ghost_map_view_igm (#et:Type) (#len: erased nat) (#st:Type0)
-  (vw : aview et len st)
+instance is_ghost_map_view_igm (#et:Type) (#st:Type0)
+  (vw : aview et st)
   : is_ghost_map st vw.iview.sch.ait et
   = vw.igm
 
 (* Nothing fancy here. *)
-let raw_view (#et:Type) (#len:nat) : aview et len (lseq et len) = {
-  iview  = IView.raw_view;
+let raw_view (#et:Type) (#len:nat) : aview et (lseq et len) = {
+  iview  = IView.raw_view #len;
   igm    = solve;
 }
 
 (* Viewing as a (ghost) function from indices to elements. Forget about sequences. *)
-let raw_function_view (#et:Type) (#len:nat) : aview et len (natlt len ^->> et) = {
-  iview  = IView.raw_view;
+let raw_function_view (#et:Type) (#len:nat) : aview et (natlt len ^->> et) = {
+  iview  = IView.raw_view #len;
   igm    = solve;
 }
 
@@ -52,8 +63,8 @@ This is typeclass already, there should be no need to mark it as a class here,
 but alas it does not quite work. *)
 inline_for_extraction noextract
 unfold
-let cview (#et : Type0) (#len : erased nat) (#st : Type0)
-  (avw : aview et len st) = IView.ciview avw.iview
+let cview (#et : Type0) (#st : Type0)
+  (avw : aview et st) = IView.ciview avw.iview
 
 let igm_reindex (#mt #it #et : Type) (igm : is_ghost_map mt it et)
   (#it': Type) (bij : it =~ it')
@@ -72,12 +83,12 @@ let igm_reindex (#mt #it #et : Type) (igm : is_ghost_map mt it et)
   l2 = ez;
 }
 
-let reindex_view (#et : Type0) (#len : nat) (#st : Type0)
-  (vw : aview et len st)
+let reindex_view (#et : Type0) (#st : Type0)
+  (vw : aview et st)
   (#ait' : Type)
   {| Enumerable.enumerable ait' |}
   (bij : vw.iview.sch.ait =~ ait')
-  : aview et len st = {
+  : aview et st = {
   iview  = IView.reindex_view vw.iview bij;
   igm    = igm_reindex vw.igm bij;
 }
@@ -93,11 +104,11 @@ let igm_review (#mt #it #et : Type) (igm : is_ghost_map mt it et)
   l2 = ez;
 }
 
-let review_view (#et : Type0) (#len : nat) (#st : Type0)
-  (vw : aview et len st)
+let review_view (#et : Type0) (#st : Type0)
+  (vw : aview et st)
   (#st' : Type)
   (bij : st =~ st')
-  : aview et len st' = {
+  : aview et st' = {
   iview    = vw.iview;
   igm      = igm_review vw.igm bij;
 }
@@ -114,30 +125,30 @@ let concrete_raw_function_view (#et:Type) (#len:nat{SZ.fits len}) : cview (raw_f
 
 (* Redefining these *)
 let it_to_nat
-  (#a:Type) (#len:nat) (#st:Type0)
-  (vw : aview a len st)
+  (#a:Type) (#st:Type0)
+  (vw : aview a st)
   (i : vw.iview.sch.ait)
-  : GTot (natlt len)
+  : GTot (natlt (len vw))
   = IView.it_to_nat vw.iview i
 
 let it_of_nat
-  (#a:Type) (#len:nat) (#st:Type0)
-  (vw : aview a len st)
-  (i: natlt len{FStar.Functions.in_image vw.iview.step.imap.f i})
+  (#a:Type) (#st:Type0)
+  (vw : aview a st)
+  (i: natlt (len vw){FStar.Functions.in_image vw.iview.step.imap.f i})
   : GTot vw.iview.sch.ait
   = IView.it_of_nat vw.iview i
 
 let ci_to_ai
-  (#et:Type) (#len:nat) (#st : Type0)
-  (vw : aview et len st)
+  (#et:Type) (#st : Type0)
+  (vw : aview et st)
   {| cw : IView.ciview vw.iview |}
   (i : cw.sch.cit)
   : GTot vw.iview.sch.ait
   = IView.ci_to_ai vw.iview i
 
 let ai_to_ci
-  (#et:Type) (#len:nat) (#st : Type0)
-  (vw : aview et len st)
+  (#et:Type) (#st : Type0)
+  (vw : aview et st)
   {| cw : IView.ciview vw.iview |}
   (i : vw.iview.sch.ait)
   : GTot cw.sch.cit
@@ -146,37 +157,38 @@ let ai_to_ci
 
 (* Operating over the abstract view. *)
 
-let is_full_view #et #len #st (vw : aview et len st) : prop =
+let is_full_view #et #st (vw : aview et st) : prop =
   IView.is_full_view vw.iview
 
 let to_seq
-  (#a:Type) (#len:nat) (#st : Type0)
-  (vw : aview a len st { is_full_view vw })
+  (#a:Type) (#st : Type0)
+  (vw : aview a st { is_full_view vw })
   (v : st)
-  : GTot (lseq a len)
-  = Seq.init_ghost len (fun i -> reveal (vw.igm.acc v (it_of_nat vw i)))
+  : GTot (lseq a (len vw))
+  = Seq.init_ghost (len vw) fun (i : natlt (len vw)) ->
+      reveal (vw.igm.acc v (it_of_nat vw i))
 
 let from_seq
-  (#a:Type) (#len:nat) (#st:Type)
-  (vw : aview a len st)
-  (s : lseq a len)
+  (#a:Type) (#st:Type)
+  (vw : aview a st)
+  (s : lseq a (len vw))
   : GTot st
   = vw.igm.bij.gg (F.on_g vw.iview.sch.ait <| fun i -> s @! it_to_nat vw i)
 
-val to_from (#a:Type) (#len:nat) (#st:Type)
-  (vw : aview a len st { is_full_view vw })
-  (s : lseq a len)
+val to_from (#a:Type) (#st:Type)
+  (vw : aview a st { is_full_view vw })
+  (s : lseq a (len vw))
   : Lemma (ensures to_seq vw (from_seq vw s) == s)
           [SMTPat (to_seq vw (from_seq vw s))]
 
-val from_to (#a:Type) (#len:nat) (#st:Type)
-  (vw : aview a len st { is_full_view vw })
+val from_to (#a:Type) (#st:Type)
+  (vw : aview a st { is_full_view vw })
   (v : st)
   : Lemma (ensures from_seq vw (to_seq vw v) == v)
           [SMTPat (from_seq vw (to_seq vw v))]
 
-val to_seq_upd (#a:Type) (#len:nat) (#st:Type)
-  (vw : aview a len st { is_full_view vw })
+val to_seq_upd (#a:Type) (#st:Type)
+  (vw : aview a st { is_full_view vw })
   (v : st)
   (i : vw.iview.sch.ait)
   (x : a)
@@ -184,11 +196,11 @@ val to_seq_upd (#a:Type) (#len:nat) (#st:Type)
           [SMTPat (to_seq vw (vw.igm.upd v i x))]
 
 let sum_aview
-  (#et : Type) (#len : nat) (#st1 #st2 : Type)
-  (vw1 : aview et len st1)
-  (vw2 : aview et len st2)
+  (#et : Type) (#st1 #st2 : Type)
+  (vw1 : aview et st1)
+  (vw2 : aview et st2)
   (#_ : squash (no_overlap vw1.iview.step.imap.f vw2.iview.step.imap.f))
-  : aview et len (st1 & st2) =
+  : aview et (st1 & st2) =
 {
   iview = sum_aiview vw1.iview vw2.iview;
   igm   = solve;
