src/lib/views/Kuiper.IView.fst
@@ -3,8 +3,7 @@ module Kuiper.IView
 #lang-pulse
 
 let full_iff_cardinal
-  (#len : nat)
-  (vw : aiview len)
-  : Lemma (is_full_view vw <==> vw.sch.ait_enum._cardinal == len)
+  (vw : aiview)
+  : Lemma (is_full_view vw <==> vw.sch.ait_enum._cardinal == vw.len)
           [SMTPat (is_full_view vw)]
   = admit()
